Push maxIdx equality into BoundedIterator

regex/Regex/Backtracker/Basic.lean
@@ -13,45 +13,44 @@ namespace Regex.Backtracker
 structure StackEntry (σ : Strategy) (nfa : NFA) (startIdx maxIdx : Nat) where
   update : σ.Update
   state : Fin nfa.nodes.size
-  it : BoundedIterator startIdx
-  eq : it.maxIdx = maxIdx
+  it : BoundedIterator startIdx maxIdx
 
 def captureNextAux (σ : Strategy) (nfa : NFA) (wf : nfa.WellFormed) (startIdx maxIdx : Nat)
   (visited : BitMatrix nfa.nodes.size (maxIdx + 1 - startIdx)) (stack : List (StackEntry σ nfa startIdx maxIdx)) :
   (Option σ.Update × BitMatrix nfa.nodes.size (maxIdx + 1 - startIdx)) :=
   match stack with
   | [] => (.none, visited)
-  | ⟨update, state, it, eq⟩ :: stack' =>
-    if h : visited.get state (it.index' eq) then
+  | ⟨update, state, it⟩ :: stack' =>
+    if h : visited.get state it.index then
       captureNextAux σ nfa wf startIdx maxIdx visited stack'
     else
-      let visited' := visited.set state (it.index' eq)
+      let visited' := visited.set state it.index
       have : nfa.nodes.size * (maxIdx + 1 - startIdx) + 1 - visited'.popcount < nfa.nodes.size * (maxIdx + 1 - startIdx) + 1 - visited.popcount :=
-        BitMatrix.popcount_decreasing visited state (it.index' eq) h
+        BitMatrix.popcount_decreasing visited state it.index h
       match hn : nfa[state] with
       | .done => (.some update, visited')
       | .fail => (.none, visited')
       | .epsilon state' =>
         have isLt : state' < nfa.nodes.size := wf.inBounds' state hn
-        captureNextAux σ nfa wf startIdx maxIdx visited' (⟨update, ⟨state', isLt⟩, it, eq⟩ :: stack')
+        captureNextAux σ nfa wf startIdx maxIdx visited' (⟨update, ⟨state', isLt⟩, it⟩ :: stack')
       | .split state₁ state₂ =>
         have isLt : state₁ < nfa.nodes.size ∧ state₂ < nfa.nodes.size := wf.inBounds' state hn
-        captureNextAux σ nfa wf startIdx maxIdx visited' (⟨update, ⟨state₁, isLt.1⟩, it, eq⟩ :: ⟨update, ⟨state₂, isLt.2⟩, it, eq⟩ :: stack')
+        captureNextAux σ nfa wf startIdx maxIdx visited' (⟨update, ⟨state₁, isLt.1⟩, it⟩ :: ⟨update, ⟨state₂, isLt.2⟩, it⟩ :: stack')
       | .save offset state' =>
         have isLt : state' < nfa.nodes.size := wf.inBounds' state hn
         let update' := σ.write update offset it.pos
-        captureNextAux σ nfa wf startIdx maxIdx visited' (⟨update', ⟨state', isLt⟩, it, eq⟩ :: stack')
+        captureNextAux σ nfa wf startIdx maxIdx visited' (⟨update', ⟨state', isLt⟩, it⟩ :: stack')
       | .anchor a state' =>
         have isLt : state' < nfa.nodes.size := wf.inBounds' state hn
         if a.test it.it then
-          captureNextAux σ nfa wf startIdx maxIdx visited' (⟨update, ⟨state', isLt⟩, it, eq⟩ :: stack')
+          captureNextAux σ nfa wf startIdx maxIdx visited' (⟨update, ⟨state', isLt⟩, it⟩ :: stack')
         else
           captureNextAux σ nfa wf startIdx maxIdx visited' stack'
       | .char c state' =>
         have isLt : state' < nfa.nodes.size := wf.inBounds' state hn
         if h : it.hasNext then
           if it.curr h = c then
-            captureNextAux σ nfa wf startIdx maxIdx visited' (⟨update, ⟨state', isLt⟩, it.next h, eq ▸ it.next_maxIdx h⟩ :: stack')
+            captureNextAux σ nfa wf startIdx maxIdx visited' (⟨update, ⟨state', isLt⟩, it.next h⟩ :: stack')
           else
             captureNextAux σ nfa wf startIdx maxIdx visited' stack'
         else
@@ -60,7 +59,7 @@ def captureNextAux (σ : Strategy) (nfa : NFA) (wf : nfa.WellFormed) (startIdx m
         have isLt : state' < nfa.nodes.size := wf.inBounds' state hn
         if h : it.hasNext then
           if it.curr h ∈ cs then
-            captureNextAux σ nfa wf startIdx maxIdx visited' (⟨update, ⟨state', isLt⟩, it.next h, eq ▸ it.next_maxIdx h⟩ :: stack')
+            captureNextAux σ nfa wf startIdx maxIdx visited' (⟨update, ⟨state', isLt⟩, it.next h⟩ :: stack')
           else
             captureNextAux σ nfa wf startIdx maxIdx visited' stack'
         else
@@ -69,20 +68,21 @@ termination_by (nfa.nodes.size * (maxIdx + 1 - startIdx) + 1 - visited.popcount,
 
 def captureNext (σ : Strategy) (nfa : NFA) (wf : nfa.WellFormed) (it : Iterator) : Option σ.Update :=
   let startIdx := it.pos.byteIdx
+  let maxIdx := it.toString.endPos.byteIdx
   if le : it.pos ≤ it.toString.endPos then
-    let bit : BoundedIterator startIdx := ⟨it, Nat.le_refl _, le⟩
-    (go startIdx bit (BitMatrix.zero _ _)).1
+    let bit : BoundedIterator startIdx maxIdx := ⟨it, Nat.le_refl _, le, rfl⟩
+    (go startIdx maxIdx bit (BitMatrix.zero _ _)).1
   else
     .none
 where
-  go (startIdx : Nat) (bit : BoundedIterator startIdx) (visited : BitMatrix nfa.nodes.size (bit.maxIdx + 1 - startIdx)) :
-  Option σ.Update × BitMatrix nfa.nodes.size (bit.maxIdx + 1 - startIdx) :=
-  match captureNextAux σ nfa wf startIdx bit.maxIdx visited [⟨σ.empty, ⟨nfa.start, wf.start_lt⟩, bit, rfl⟩] with
+  go (startIdx maxIdx : Nat) (bit : BoundedIterator startIdx maxIdx) (visited : BitMatrix nfa.nodes.size (maxIdx + 1 - startIdx)) :
+  Option σ.Update × BitMatrix nfa.nodes.size (maxIdx + 1 - startIdx) :=
+  match captureNextAux σ nfa wf startIdx maxIdx visited [⟨σ.empty, ⟨nfa.start, wf.start_lt⟩, bit⟩] with
   | (.some update, visited') => (.some update, visited')
   | (.none, visited') =>
     if h : bit.hasNext then
       have : (bit.next h).remainingBytes < bit.remainingBytes := bit.next_remainingBytes_lt h
-      go startIdx (bit.next h) visited'
+      go startIdx maxIdx (bit.next h) visited'
     else
       (.none, visited')
   termination_by bit.remainingBytes
