correctness/RegexCorrectness/Backtracker/Basic.lean
@@ -11,177 +11,177 @@ theorem captureNextAux.induct' (σ : Strategy) (nfa : NFA) (wf : nfa.WellFormed)
   (base : ∀ (visited : BitMatrix nfa.nodes.size (maxIdx + 1 - startIdx)), motive visited [])
   (visited :
     ∀ (visited : BitMatrix nfa.nodes.size (maxIdx + 1 - startIdx)) (update : σ.Update)
-      (state : Fin nfa.nodes.size) (it : BoundedIterator startIdx) (eq : it.maxIdx = maxIdx)
+      (state : Fin nfa.nodes.size) (it : BoundedIterator startIdx maxIdx)
       (stack' : List (StackEntry σ nfa startIdx maxIdx)),
-    visited.get state (it.index' eq) →
+    visited.get state it.index →
     motive visited stack' →
-    motive visited (⟨update, state, it, eq⟩ :: stack'))
+    motive visited (⟨update, state, it⟩ :: stack'))
   (done :
     ∀ (visited : BitMatrix nfa.nodes.size (maxIdx + 1 - startIdx)) (update : σ.Update)
-      (state : Fin nfa.nodes.size) (it : BoundedIterator startIdx) (eq : it.maxIdx = maxIdx)
+      (state : Fin nfa.nodes.size) (it : BoundedIterator startIdx maxIdx)
       (stack' : List (StackEntry σ nfa startIdx maxIdx)),
-    ¬visited.get state (it.index' eq) →
+    ¬visited.get state it.index →
     nfa[state] = NFA.Node.done →
-    motive visited (⟨update, state, it, eq⟩ :: stack'))
+    motive visited (⟨update, state, it⟩ :: stack'))
   (fail :
     ∀ (visited : BitMatrix nfa.nodes.size (maxIdx + 1 - startIdx)) (update : σ.Update)
-      (state : Fin nfa.nodes.size) (it : BoundedIterator startIdx) (eq : it.maxIdx = maxIdx)
+      (state : Fin nfa.nodes.size) (it : BoundedIterator startIdx maxIdx)
       (stack' : List (StackEntry σ nfa startIdx maxIdx)),
-    ¬visited.get state (it.index' eq) →
+    ¬visited.get state it.index →
     nfa[state] = NFA.Node.fail →
-    motive visited (⟨update, state, it, eq⟩ :: stack'))
+    motive visited (⟨update, state, it⟩ :: stack'))
   (epsilon :
     ∀ (visited : BitMatrix nfa.nodes.size (maxIdx + 1 - startIdx)) (update : σ.Update)
-      (state : Fin nfa.nodes.size) (it : BoundedIterator startIdx) (eq : it.maxIdx = maxIdx)
+      (state : Fin nfa.nodes.size) (it : BoundedIterator startIdx maxIdx)
       (stack' : List (StackEntry σ nfa startIdx maxIdx)),
-    ¬visited.get state (it.index' eq) →
-    let visited' := visited.set state (it.index' eq);
+    ¬visited.get state it.index →
+    let visited' := visited.set state it.index;
     ∀ (state' : Fin nfa.nodes.size),
     nfa[state] = NFA.Node.epsilon state' →
-    motive visited' (⟨update, state', it, eq⟩ :: stack') →
-    motive visited (⟨update, state, it, eq⟩ :: stack'))
+    motive visited' (⟨update, state', it⟩ :: stack') →
+    motive visited (⟨update, state, it⟩ :: stack'))
   (split :
     ∀ (visited : BitMatrix nfa.nodes.size (maxIdx + 1 - startIdx)) (update : σ.Update)
-      (state : Fin nfa.nodes.size) (it : BoundedIterator startIdx) (eq : it.maxIdx = maxIdx)
+      (state : Fin nfa.nodes.size) (it : BoundedIterator startIdx maxIdx)
       (stack' : List (StackEntry σ nfa startIdx maxIdx)),
-    ¬visited.get state (it.index' eq) →
-    let visited' := visited.set state (it.index' eq);
+    ¬visited.get state it.index →
+    let visited' := visited.set state it.index;
     ∀ (state₁ state₂ : Fin nfa.nodes.size),
     nfa[state] = NFA.Node.split state₁ state₂ →
-    motive visited' (⟨update, state₁, it, eq⟩ :: ⟨update, state₂, it, eq⟩ :: stack') →
-    motive visited (⟨update, state, it, eq⟩ :: stack'))
+    motive visited' (⟨update, state₁, it⟩ :: ⟨update, state₂, it⟩ :: stack') →
+    motive visited (⟨update, state, it⟩ :: stack'))
   (save :
     ∀ (visited : BitMatrix nfa.nodes.size (maxIdx + 1 - startIdx)) (update : σ.Update)
-      (state : Fin nfa.nodes.size) (it : BoundedIterator startIdx) (eq : it.maxIdx = maxIdx)
+      (state : Fin nfa.nodes.size) (it : BoundedIterator startIdx maxIdx)
       (stack' : List (StackEntry σ nfa startIdx maxIdx)),
-    ¬visited.get state (it.index' eq) →
-    let visited' := visited.set state (it.index' eq);
+    ¬visited.get state it.index →
+    let visited' := visited.set state it.index;
     ∀ (offset : Nat) (state' : Fin nfa.nodes.size),
     nfa[state] = NFA.Node.save offset state' →
     let update' := σ.write update offset it.pos;
-    motive visited' (⟨update', state', it, eq⟩ :: stack') →
-    motive visited (⟨update, state, it, eq⟩ :: stack'))
+    motive visited' (⟨update', state', it⟩ :: stack') →
+    motive visited (⟨update, state, it⟩ :: stack'))
   (anchor_pos :
     ∀ (visited : BitMatrix nfa.nodes.size (maxIdx + 1 - startIdx)) (update : σ.Update)
-      (state : Fin nfa.nodes.size) (it : BoundedIterator startIdx) (eq : it.maxIdx = maxIdx)
+      (state : Fin nfa.nodes.size) (it : BoundedIterator startIdx maxIdx)
       (stack' : List (StackEntry σ nfa startIdx maxIdx)),
-    ¬visited.get state (it.index' eq) →
-    let visited' := visited.set state (it.index' eq);
+    ¬visited.get state it.index →
+    let visited' := visited.set state it.index;
     ∀ (a : Data.Anchor) (state' : Fin nfa.nodes.size),
     nfa[state] = NFA.Node.anchor a state' →
     Data.Anchor.test it.it a →
-    motive visited' (⟨update, state', it, eq⟩ :: stack') →
-    motive visited (⟨update, state, it, eq⟩ :: stack'))
+    motive visited' (⟨update, state', it⟩ :: stack') →
+    motive visited (⟨update, state, it⟩ :: stack'))
   (anchor_neg :
     ∀ (visited : BitMatrix nfa.nodes.size (maxIdx + 1 - startIdx)) (update : σ.Update)
-      (state : Fin nfa.nodes.size) (it : BoundedIterator startIdx) (eq : it.maxIdx = maxIdx)
+      (state : Fin nfa.nodes.size) (it : BoundedIterator startIdx maxIdx)
       (stack' : List (StackEntry σ nfa startIdx maxIdx)),
-    ¬visited.get state (it.index' eq) →
-    let visited' := visited.set state (it.index' eq);
+    ¬visited.get state it.index →
+    let visited' := visited.set state it.index;
     ∀ (a : Data.Anchor) (state' : Fin nfa.nodes.size),
     nfa[state] = NFA.Node.anchor a state' →
     ¬Data.Anchor.test it.it a →
     motive visited' stack' →
-    motive visited (⟨update, state, it, eq⟩ :: stack'))
+    motive visited (⟨update, state, it⟩ :: stack'))
   (char_pos :
     ∀ (visited : BitMatrix nfa.nodes.size (maxIdx + 1 - startIdx)) (update : σ.Update)
-      (state : Fin nfa.nodes.size) (it : BoundedIterator startIdx) (eq : it.maxIdx = maxIdx)
+      (state : Fin nfa.nodes.size) (it : BoundedIterator startIdx maxIdx)
       (stack' : List (StackEntry σ nfa startIdx maxIdx)),
-    ¬visited.get state (it.index' eq) →
-    let visited' := visited.set state (it.index' eq);
+    ¬visited.get state it.index →
+    let visited' := visited.set state it.index;
     ∀ (c : Char) (state' : Fin nfa.nodes.size),
     nfa[state] = NFA.Node.char c state' →
     (h : it.hasNext) →
     it.curr h = c →
-    motive visited' (⟨update, state', it.next h, eq⟩ :: stack') →
-    motive visited (⟨update, state, it, eq⟩ :: stack'))
+    motive visited' (⟨update, state', it.next h⟩ :: stack') →
+    motive visited (⟨update, state, it⟩ :: stack'))
   (char_neg :
     ∀ (visited : BitMatrix nfa.nodes.size (maxIdx + 1 - startIdx)) (update : σ.Update)
-      (state : Fin nfa.nodes.size) (it : BoundedIterator startIdx) (eq : it.maxIdx = maxIdx)
+      (state : Fin nfa.nodes.size) (it : BoundedIterator startIdx maxIdx)
       (stack' : List (StackEntry σ nfa startIdx maxIdx)),
-    ¬visited.get state (it.index' eq) →
-    let visited' := visited.set state (it.index' eq);
+    ¬visited.get state it.index →
+    let visited' := visited.set state it.index;
     ∀ (c : Char) (state' : Fin nfa.nodes.size),
     nfa[state] = NFA.Node.char c state' →
     (h : it.hasNext) →
     ¬it.curr h = c →
     motive visited' stack' →
-    motive visited (⟨update, state, it, eq⟩ :: stack'))
+    motive visited (⟨update, state, it⟩ :: stack'))
   (char_end :
     ∀ (visited : BitMatrix nfa.nodes.size (maxIdx + 1 - startIdx)) (update : σ.Update)
-      (state : Fin nfa.nodes.size) (it : BoundedIterator startIdx) (eq : it.maxIdx = maxIdx)
+      (state : Fin nfa.nodes.size) (it : BoundedIterator startIdx maxIdx)
       (stack' : List (StackEntry σ nfa startIdx maxIdx)),
-    ¬visited.get state (it.index' eq) →
-    let visited' := visited.set state (it.index' eq);
+    ¬visited.get state it.index →
+    let visited' := visited.set state it.index;
     ∀ (c : Char) (state' : Fin nfa.nodes.size),
     nfa[state] = NFA.Node.char c state' →
     ¬it.hasNext →
     motive visited' stack' →
-    motive visited (⟨update, state, it, eq⟩ :: stack'))
+    motive visited (⟨update, state, it⟩ :: stack'))
   (sparse_pos :
     ∀ (visited : BitMatrix nfa.nodes.size (maxIdx + 1 - startIdx)) (update : σ.Update)
-      (state : Fin nfa.nodes.size) (it : BoundedIterator startIdx) (eq : it.maxIdx = maxIdx)
+      (state : Fin nfa.nodes.size) (it : BoundedIterator startIdx maxIdx)
       (stack' : List (StackEntry σ nfa startIdx maxIdx)),
-    ¬visited.get state (it.index' eq) →
-    let visited' := visited.set state (it.index' eq);
+    ¬visited.get state it.index →
+    let visited' := visited.set state it.index;
     ∀ (cs : Data.Classes) (state' : Fin nfa.nodes.size),
     nfa[state] = NFA.Node.sparse cs state' →
     (h : it.hasNext) →
     it.curr h ∈ cs →
-    motive visited' (⟨update, state', it.next h, eq⟩ :: stack') →
-    motive visited (⟨update, state, it, eq⟩ :: stack'))
+    motive visited' (⟨update, state', it.next h⟩ :: stack') →
+    motive visited (⟨update, state, it⟩ :: stack'))
   (sparse_neg :
     ∀ (visited : BitMatrix nfa.nodes.size (maxIdx + 1 - startIdx)) (update : σ.Update)
-      (state : Fin nfa.nodes.size) (it : BoundedIterator startIdx) (eq : it.maxIdx = maxIdx)
+      (state : Fin nfa.nodes.size) (it : BoundedIterator startIdx maxIdx)
       (stack' : List (StackEntry σ nfa startIdx maxIdx)),
-    ¬visited.get state (it.index' eq) →
-    let visited' := visited.set state (it.index' eq);
+    ¬visited.get state it.index →
+    let visited' := visited.set state it.index;
     ∀ (cs : Data.Classes) (state' : Fin nfa.nodes.size),
     nfa[state] = NFA.Node.sparse cs state' →
     (h : it.hasNext) →
     ¬it.curr h ∈ cs →
     motive visited' stack' →
-    motive visited (⟨update, state, it, eq⟩ :: stack'))
+    motive visited (⟨update, state, it⟩ :: stack'))
   (sparse_end :
     ∀ (visited : BitMatrix nfa.nodes.size (maxIdx + 1 - startIdx)) (update : σ.Update)
-      (state : Fin nfa.nodes.size) (it : BoundedIterator startIdx) (eq : it.maxIdx = maxIdx)
+      (state : Fin nfa.nodes.size) (it : BoundedIterator startIdx maxIdx)
       (stack' : List (StackEntry σ nfa startIdx maxIdx)),
-    ¬visited.get state (it.index' eq) →
-    let visited' := visited.set state (it.index' eq);
+    ¬visited.get state it.index →
+    let visited' := visited.set state it.index;
     ∀ (cs : Data.Classes) (state' : Fin nfa.nodes.size),
     nfa[state] = NFA.Node.sparse cs state' →
     ¬it.hasNext →
     motive visited' stack' →
-    motive visited (⟨update, state, it, eq⟩ :: stack'))
+    motive visited (⟨update, state, it⟩ :: stack'))
   (matrix : BitMatrix nfa.nodes.size (maxIdx + 1 - startIdx)) (stack : List (StackEntry σ nfa startIdx maxIdx)) :
   motive matrix stack :=
   captureNextAux.induct σ nfa wf startIdx maxIdx motive base visited
-    (fun visited update state it eq stack' mem _ hn =>
-      done visited update state it eq stack' mem hn)
-    (fun visited update state it eq stack' mem _ hn =>
-      fail visited update state it eq stack' mem hn)
-    (fun visited update state it eq stack' mem _ state' hn isLt ih =>
-      epsilon visited update state it eq stack' mem ⟨state', isLt⟩ hn ih)
-    (fun visited update state it eq stack' mem _ state₁ state₂ hn isLt ih =>
-      split visited update state it eq stack' mem ⟨state₁, isLt.1⟩ ⟨state₂, isLt.2⟩ hn ih)
-    (fun visited update state it eq stack' mem _ offset state' hn isLt ih =>
-      save visited update state it eq stack' mem offset ⟨state', isLt⟩ hn ih)
-    (fun visited update state it eq stack' mem _ a state' hn isLt ih =>
-      anchor_pos visited update state it eq stack' mem a ⟨state', isLt⟩ hn ih)
-    (fun visited update state it eq stack' mem _ a state' hn isLt ih =>
-      anchor_neg visited update state it eq stack' mem a ⟨state', isLt⟩ hn ih)
-    (fun visited update state it eq stack' mem _ state' isLt h hn ih =>
-      char_pos visited update state it eq stack' mem (it.curr h) ⟨state', isLt⟩ hn h rfl ih)
-    (fun visited update state it eq stack' mem _ c state' hn isLt h ne ih =>
-      char_neg visited update state it eq stack' mem c ⟨state', isLt⟩ hn h ne ih)
-    (fun visited update state it eq stack' mem _ c state' hn isLt h ih =>
-      char_end visited update state it eq stack' mem c ⟨state', isLt⟩ hn h ih)
-    (fun visited update state it eq stack' mem _ cs state' hn isLt h ih =>
-      sparse_pos visited update state it eq stack' mem cs ⟨state', isLt⟩ hn h ih)
-    (fun visited update state it eq stack' mem _ cs state' hn isLt h ih =>
-      sparse_neg visited update state it eq stack' mem cs ⟨state', isLt⟩ hn h ih)
-    (fun visited update state it eq stack' mem _ cs state' hn isLt h ih =>
-      sparse_end visited update state it eq stack' mem cs ⟨state', isLt⟩ hn h ih)
+    (fun visited update state it stack' mem _ hn =>
+      done visited update state it stack' mem hn)
+    (fun visited update state it stack' mem _ hn =>
+      fail visited update state it stack' mem hn)
+    (fun visited update state it stack' mem _ state' hn isLt ih =>
+      epsilon visited update state it stack' mem ⟨state', isLt⟩ hn ih)
+    (fun visited update state it stack' mem _ state₁ state₂ hn isLt ih =>
+      split visited update state it stack' mem ⟨state₁, isLt.1⟩ ⟨state₂, isLt.2⟩ hn ih)
+    (fun visited update state it stack' mem _ offset state' hn isLt ih =>
+      save visited update state it stack' mem offset ⟨state', isLt⟩ hn ih)
+    (fun visited update state it stack' mem _ a state' hn isLt ih =>
+      anchor_pos visited update state it stack' mem a ⟨state', isLt⟩ hn ih)
+    (fun visited update state it stack' mem _ a state' hn isLt ih =>
+      anchor_neg visited update state it stack' mem a ⟨state', isLt⟩ hn ih)
+    (fun visited update state it stack' mem _ state' isLt h hn ih =>
+      char_pos visited update state it stack' mem (it.curr h) ⟨state', isLt⟩ hn h rfl ih)
+    (fun visited update state it stack' mem _ c state' hn isLt h ne ih =>
+      char_neg visited update state it stack' mem c ⟨state', isLt⟩ hn h ne ih)
+    (fun visited update state it stack' mem _ c state' hn isLt h ih =>
+      char_end visited update state it stack' mem c ⟨state', isLt⟩ hn h ih)
+    (fun visited update state it stack' mem _ cs state' hn isLt h ih =>
+      sparse_pos visited update state it stack' mem cs ⟨state', isLt⟩ hn h ih)
+    (fun visited update state it stack' mem _ cs state' hn isLt h ih =>
+      sparse_neg visited update state it stack' mem cs ⟨state', isLt⟩ hn h ih)
+    (fun visited update state it stack' mem _ cs state' hn isLt h ih =>
+      sparse_end visited update state it stack' mem cs ⟨state', isLt⟩ hn h ih)
     matrix stack
 
 /-
@@ -195,15 +195,15 @@ theorem captureNextAux_base :
   captureNextAux σ nfa wf startIdx maxIdx visited [] = (.none, visited) := by
   simp [captureNextAux]
 
-theorem captureNextAux_visited {update state it eq stack'} (mem : visited.get state (it.index' eq)) :
-  captureNextAux σ nfa wf startIdx maxIdx visited (⟨update, state, it, eq⟩ :: stack') = captureNextAux σ nfa wf startIdx maxIdx visited stack' := by
+theorem captureNextAux_visited {update state it stack'} (mem : visited.get state it.index) :
+  captureNextAux σ nfa wf startIdx maxIdx visited (⟨update, state, it⟩ :: stack') = captureNextAux σ nfa wf startIdx maxIdx visited stack' := by
   conv =>
     lhs
     unfold captureNextAux
     simp [mem]
 
-theorem captureNextAux_done {update state it eq stack'} (mem : ¬visited.get state (it.index' eq)) (hn : nfa[state] = .done) :
-  captureNextAux σ nfa wf startIdx maxIdx visited (⟨update, state, it, eq⟩ :: stack') = (.some update, visited.set state (it.index' eq)) := by
+theorem captureNextAux_done {update state it stack'} (mem : ¬visited.get state it.index) (hn : nfa[state] = .done) :
+  captureNextAux σ nfa wf startIdx maxIdx visited (⟨update, state, it⟩ :: stack') = (.some update, visited.set state it.index) := by
   simp at hn
   conv =>
     lhs
@@ -211,107 +211,107 @@ theorem captureNextAux_done {update state it eq stack'} (mem : ¬visited.get sta
     simp [mem]
   split <;> simp_all
 
-theorem captureNextAux_fail {update state it eq stack'} (mem : ¬visited.get state (it.index' eq)) (hn : nfa[state] = .fail) :
-  captureNextAux σ nfa wf startIdx maxIdx visited (⟨update, state, it, eq⟩ :: stack') = (.none, visited.set state (it.index' eq)) := by
+theorem captureNextAux_fail {update state it stack'} (mem : ¬visited.get state it.index) (hn : nfa[state] = .fail) :
+  captureNextAux σ nfa wf startIdx maxIdx visited (⟨update, state, it⟩ :: stack') = (.none, visited.set state it.index) := by
   conv =>
     lhs
     unfold captureNextAux
     simp [mem]
   split <;> simp_all
 
-theorem captureNextAux_epsilon {update state it eq stack' state'} (mem : ¬visited.get state (it.index' eq)) (hn : nfa[state] = .epsilon state') :
-  captureNextAux σ nfa wf startIdx maxIdx visited (⟨update, state, it, eq⟩ :: stack') =
-  captureNextAux σ nfa wf startIdx maxIdx (visited.set state (it.index' eq)) (⟨update, state', it, eq⟩ :: stack') := by
+theorem captureNextAux_epsilon {update state it stack' state'} (mem : ¬visited.get state it.index) (hn : nfa[state] = .epsilon state') :
+  captureNextAux σ nfa wf startIdx maxIdx visited (⟨update, state, it⟩ :: stack') =
+  captureNextAux σ nfa wf startIdx maxIdx (visited.set state it.index) (⟨update, state', it⟩ :: stack') := by
   conv =>
     lhs
     unfold captureNextAux
     simp [mem]
   split <;> simp_all
 
-theorem captureNextAux_split {update state it eq stack' state₁ state₂} (mem : ¬visited.get state (it.index' eq)) (hn : nfa[state] = .split state₁ state₂) :
-  captureNextAux σ nfa wf startIdx maxIdx visited (⟨update, state, it, eq⟩ :: stack') =
-  captureNextAux σ nfa wf startIdx maxIdx (visited.set state (it.index' eq)) (⟨update, state₁, it, eq⟩ :: ⟨update, state₂, it, eq⟩ :: stack') := by
+theorem captureNextAux_split {update state it stack' state₁ state₂} (mem : ¬visited.get state it.index) (hn : nfa[state] = .split state₁ state₂) :
+  captureNextAux σ nfa wf startIdx maxIdx visited (⟨update, state, it⟩ :: stack') =
+  captureNextAux σ nfa wf startIdx maxIdx (visited.set state it.index) (⟨update, state₁, it⟩ :: ⟨update, state₂, it⟩ :: stack') := by
   conv =>
     lhs
     unfold captureNextAux
     simp [mem]
   split <;> simp_all
 
-theorem captureNextAux_save {update state it eq stack' offset state'} (mem : ¬visited.get state (it.index' eq)) (hn : nfa[state] = .save offset state') :
-  captureNextAux σ nfa wf startIdx maxIdx visited (⟨update, state, it, eq⟩ :: stack') =
-  captureNextAux σ nfa wf startIdx maxIdx (visited.set state (it.index' eq)) (⟨σ.write update offset it.pos, state', it, eq⟩ :: stack') := by
+theorem captureNextAux_save {update state it stack' offset state'} (mem : ¬visited.get state it.index) (hn : nfa[state] = .save offset state') :
+  captureNextAux σ nfa wf startIdx maxIdx visited (⟨update, state, it⟩ :: stack') =
+  captureNextAux σ nfa wf startIdx maxIdx (visited.set state it.index) (⟨σ.write update offset it.pos, state', it⟩ :: stack') := by
   conv =>
     lhs
     unfold captureNextAux
     simp [mem]
   split <;> simp_all
 
-theorem captureNextAux_anchor_pos {update state it eq stack' a state'} (mem : ¬visited.get state (it.index' eq)) (hn : nfa[state] = .anchor a state') (h : Data.Anchor.test it.it a) :
-  captureNextAux σ nfa wf startIdx maxIdx visited (⟨update, state, it, eq⟩ :: stack') =
-  captureNextAux σ nfa wf startIdx maxIdx (visited.set state (it.index' eq)) (⟨update, state', it, eq⟩ :: stack') := by
+theorem captureNextAux_anchor_pos {update state it stack' a state'} (mem : ¬visited.get state it.index) (hn : nfa[state] = .anchor a state') (h : Data.Anchor.test it.it a) :
+  captureNextAux σ nfa wf startIdx maxIdx visited (⟨update, state, it⟩ :: stack') =
+  captureNextAux σ nfa wf startIdx maxIdx (visited.set state it.index) (⟨update, state', it⟩ :: stack') := by
   conv =>
     lhs
     unfold captureNextAux
     simp [mem]
   split <;> simp_all
 
-theorem captureNextAux_anchor_neg {update state it eq stack' a state'} (mem : ¬visited.get state (it.index' eq)) (hn : nfa[state] = .anchor a state') (h : ¬Data.Anchor.test it.it a) :
-  captureNextAux σ nfa wf startIdx maxIdx visited (⟨update, state, it, eq⟩ :: stack') =
-  captureNextAux σ nfa wf startIdx maxIdx (visited.set state (it.index' eq)) stack' := by
+theorem captureNextAux_anchor_neg {update state it stack' a state'} (mem : ¬visited.get state it.index) (hn : nfa[state] = .anchor a state') (h : ¬Data.Anchor.test it.it a) :
+  captureNextAux σ nfa wf startIdx maxIdx visited (⟨update, state, it⟩ :: stack') =
+  captureNextAux σ nfa wf startIdx maxIdx (visited.set state it.index) stack' := by
   conv =>
     lhs
     unfold captureNextAux
     simp [mem]
   split <;> simp_all
 
-theorem captureNextAux_char_pos {update state it eq stack' c state'} (mem : ¬visited.get state (it.index' eq)) (hn : nfa[state] = .char c state') (h : it.hasNext) (hc : it.curr h = c) :
-  captureNextAux σ nfa wf startIdx maxIdx visited (⟨update, state, it, eq⟩ :: stack') =
-  captureNextAux σ nfa wf startIdx maxIdx (visited.set state (it.index' eq)) (⟨update, state', it.next h, eq⟩ :: stack') := by
+theorem captureNextAux_char_pos {update state it stack' c state'} (mem : ¬visited.get state it.index) (hn : nfa[state] = .char c state') (h : it.hasNext) (hc : it.curr h = c) :
+  captureNextAux σ nfa wf startIdx maxIdx visited (⟨update, state, it⟩ :: stack') =
+  captureNextAux σ nfa wf startIdx maxIdx (visited.set state it.index) (⟨update, state', it.next h⟩ :: stack') := by
   conv =>
     lhs
     unfold captureNextAux
     simp [mem]
   split <;> simp_all
 
-theorem captureNextAux_char_neg {update state it eq stack' c state'} (mem : ¬visited.get state (it.index' eq)) (hn : nfa[state] = .char c state') (h : it.hasNext) (hc : ¬it.curr h = c) :
-  captureNextAux σ nfa wf startIdx maxIdx visited (⟨update, state, it, eq⟩ :: stack') =
-  captureNextAux σ nfa wf startIdx maxIdx (visited.set state (it.index' eq)) stack' := by
+theorem captureNextAux_char_neg {update state it stack' c state'} (mem : ¬visited.get state it.index) (hn : nfa[state] = .char c state') (h : it.hasNext) (hc : ¬it.curr h = c) :
+  captureNextAux σ nfa wf startIdx maxIdx visited (⟨update, state, it⟩ :: stack') =
+  captureNextAux σ nfa wf startIdx maxIdx (visited.set state it.index) stack' := by
   conv =>
     lhs
     unfold captureNextAux
     simp [mem]
   split <;> simp_all
 
-theorem captureNextAux_char_end {update state it eq stack' c state'} (mem : ¬visited.get state (it.index' eq)) (hn : nfa[state] = .char c state') (h : ¬it.hasNext) :
-  captureNextAux σ nfa wf startIdx maxIdx visited (⟨update, state, it, eq⟩ :: stack') =
-  captureNextAux σ nfa wf startIdx maxIdx (visited.set state (it.index' eq)) stack' := by
+theorem captureNextAux_char_end {update state it stack' c state'} (mem : ¬visited.get state it.index) (hn : nfa[state] = .char c state') (h : ¬it.hasNext) :
+  captureNextAux σ nfa wf startIdx maxIdx visited (⟨update, state, it⟩ :: stack') =
+  captureNextAux σ nfa wf startIdx maxIdx (visited.set state it.index) stack' := by
   conv =>
     lhs
     unfold captureNextAux
     simp [mem]
   split <;> simp_all
 
-theorem captureNextAux_sparse_pos {update state it eq stack' cs state'} (mem : ¬visited.get state (it.index' eq)) (hn : nfa[state] = .sparse cs state') (h : it.hasNext) (hc : it.curr h ∈ cs) :
-  captureNextAux σ nfa wf startIdx maxIdx visited (⟨update, state, it, eq⟩ :: stack') =
-  captureNextAux σ nfa wf startIdx maxIdx (visited.set state (it.index' eq)) (⟨update, state', it.next h, eq⟩ :: stack') := by
+theorem captureNextAux_sparse_pos {update state it stack' cs state'} (mem : ¬visited.get state it.index) (hn : nfa[state] = .sparse cs state') (h : it.hasNext) (hc : it.curr h ∈ cs) :
+  captureNextAux σ nfa wf startIdx maxIdx visited (⟨update, state, it⟩ :: stack') =
+  captureNextAux σ nfa wf startIdx maxIdx (visited.set state it.index) (⟨update, state', it.next h⟩ :: stack') := by
   conv =>
     lhs
     unfold captureNextAux
     simp [mem]
   split <;> simp_all
 
-theorem captureNextAux_sparse_neg {update state it eq stack' cs state'} (mem : ¬visited.get state (it.index' eq)) (hn : nfa[state] = .sparse cs state') (h : it.hasNext) (hc : ¬it.curr h ∈ cs) :
-  captureNextAux σ nfa wf startIdx maxIdx visited (⟨update, state, it, eq⟩ :: stack') =
-  captureNextAux σ nfa wf startIdx maxIdx (visited.set state (it.index' eq)) stack' := by
+theorem captureNextAux_sparse_neg {update state it stack' cs state'} (mem : ¬visited.get state it.index) (hn : nfa[state] = .sparse cs state') (h : it.hasNext) (hc : ¬it.curr h ∈ cs) :
+  captureNextAux σ nfa wf startIdx maxIdx visited (⟨update, state, it⟩ :: stack') =
+  captureNextAux σ nfa wf startIdx maxIdx (visited.set state it.index) stack' := by
   conv =>
     lhs
     unfold captureNextAux
     simp [mem]
   split <;> simp_all
 
-theorem captureNextAux_sparse_end {update state it eq stack' cs state'} (mem : ¬visited.get state (it.index' eq)) (hn : nfa[state] = .sparse cs state') (h : ¬it.hasNext) :
-  captureNextAux σ nfa wf startIdx maxIdx visited (⟨update, state, it, eq⟩ :: stack') =
-  captureNextAux σ nfa wf startIdx maxIdx (visited.set state (it.index' eq)) stack' := by
+theorem captureNextAux_sparse_end {update state it stack' cs state'} (mem : ¬visited.get state it.index) (hn : nfa[state] = .sparse cs state') (h : ¬it.hasNext) :
+  captureNextAux σ nfa wf startIdx maxIdx visited (⟨update, state, it⟩ :: stack') =
+  captureNextAux σ nfa wf startIdx maxIdx (visited.set state it.index) stack' := by
   conv =>
     lhs
     unfold captureNextAux
@@ -320,23 +320,23 @@ theorem captureNextAux_sparse_end {update state it eq stack' cs state'} (mem : �
 
 end
 
-theorem captureNext.go.induct' (σ : Strategy) (nfa : NFA) (wf : nfa.WellFormed) (startIdx : Nat)
-  (motive : (bit : BoundedIterator startIdx) → BitMatrix nfa.nodes.size (bit.maxIdx + 1 - startIdx) → Prop)
-  (found : ∀ (bit : BoundedIterator startIdx) (visited : BitMatrix nfa.nodes.size (bit.maxIdx + 1 - startIdx)) (update : σ.Update) (visited' : BitMatrix nfa.nodes.size (bit.maxIdx + 1 - startIdx)),
-    captureNextAux σ nfa wf startIdx bit.maxIdx visited [⟨σ.empty, ⟨nfa.start, wf.start_lt⟩, bit, rfl⟩] = (.some update, visited') →
+theorem captureNext.go.induct' (σ : Strategy) (nfa : NFA) (wf : nfa.WellFormed) (startIdx maxIdx : Nat)
+  (motive : (bit : BoundedIterator startIdx maxIdx) → BitMatrix nfa.nodes.size (maxIdx + 1 - startIdx) → Prop)
+  (found : ∀ (bit : BoundedIterator startIdx maxIdx) (visited : BitMatrix nfa.nodes.size (maxIdx + 1 - startIdx)) (update : σ.Update) (visited' : BitMatrix nfa.nodes.size (maxIdx + 1 - startIdx)),
+    captureNextAux σ nfa wf startIdx maxIdx visited [⟨σ.empty, ⟨nfa.start, wf.start_lt⟩, bit⟩] = (.some update, visited') →
     motive bit visited)
-  (not_found_next : ∀ (bit : BoundedIterator startIdx) (visited visited' : BitMatrix nfa.nodes.size (bit.maxIdx + 1 - startIdx)),
-    captureNextAux σ nfa wf startIdx bit.maxIdx visited [⟨σ.empty, ⟨nfa.start, wf.start_lt⟩, bit, rfl⟩] = (.none, visited') →
+  (not_found_next : ∀ (bit : BoundedIterator startIdx maxIdx) (visited visited' : BitMatrix nfa.nodes.size (maxIdx + 1 - startIdx)),
+    captureNextAux σ nfa wf startIdx maxIdx visited [⟨σ.empty, ⟨nfa.start, wf.start_lt⟩, bit⟩] = (.none, visited') →
     (h : bit.hasNext) →
     (ih : motive (bit.next h) visited') →
     motive bit visited)
-  (not_found_end : ∀ (bit : BoundedIterator startIdx) (visited visited' : BitMatrix nfa.nodes.size (bit.maxIdx + 1 - startIdx)),
-    captureNextAux σ nfa wf startIdx bit.maxIdx visited [⟨σ.empty, ⟨nfa.start, wf.start_lt⟩, bit, rfl⟩] = (.none, visited') →
+  (not_found_end : ∀ (bit : BoundedIterator startIdx maxIdx) (visited visited' : BitMatrix nfa.nodes.size (maxIdx + 1 - startIdx)),
+    captureNextAux σ nfa wf startIdx maxIdx visited [⟨σ.empty, ⟨nfa.start, wf.start_lt⟩, bit⟩] = (.none, visited') →
     ¬bit.hasNext →
     motive bit visited)
-  (bit : BoundedIterator startIdx) (visited : BitMatrix nfa.nodes.size (bit.maxIdx + 1 - startIdx)) :
+  (bit : BoundedIterator startIdx maxIdx) (visited : BitMatrix nfa.nodes.size (maxIdx + 1 - startIdx)) :
   motive bit visited :=
-  captureNext.go.induct σ nfa wf startIdx motive
+  captureNext.go.induct σ nfa wf startIdx maxIdx motive
     found
     (fun bit visited visited' hres h _ ih => not_found_next bit visited visited' hres h ih)
     not_found_end
@@ -347,22 +347,22 @@ Simplification lemmas for `captureNext.go`.
 -/
 section
 
-variable {σ nfa wf startIdx bit visited}
+variable {σ nfa wf startIdx maxIdx bit visited}
 
-theorem captureNext.go_found {update visited'} (h : captureNextAux σ nfa wf startIdx bit.maxIdx visited [⟨σ.empty, ⟨nfa.start, wf.start_lt⟩, bit, rfl⟩] = (.some update, visited')) :
-  captureNext.go σ nfa wf startIdx bit visited = (.some update, visited') := by
+theorem captureNext.go_found {update visited'} (h : captureNextAux σ nfa wf startIdx maxIdx visited [⟨σ.empty, ⟨nfa.start, wf.start_lt⟩, bit⟩] = (.some update, visited')) :
+  captureNext.go σ nfa wf startIdx maxIdx bit visited = (.some update, visited') := by
   unfold captureNext.go
   split <;> simp_all
 
-theorem captureNext.go_not_found_next {visited'} (h : captureNextAux σ nfa wf startIdx bit.maxIdx visited [⟨σ.empty, ⟨nfa.start, wf.start_lt⟩, bit, rfl⟩] = (.none, visited')) (h' : bit.hasNext) :
-  captureNext.go σ nfa wf startIdx bit visited = captureNext.go σ nfa wf startIdx (bit.next h') visited' := by
+theorem captureNext.go_not_found_next {visited'} (h : captureNextAux σ nfa wf startIdx maxIdx visited [⟨σ.empty, ⟨nfa.start, wf.start_lt⟩, bit⟩] = (.none, visited')) (h' : bit.hasNext) :
+  captureNext.go σ nfa wf startIdx maxIdx bit visited = captureNext.go σ nfa wf startIdx maxIdx (bit.next h') visited' := by
   conv =>
     lhs
     unfold captureNext.go
   split <;> simp_all
 
-theorem captureNext.go_not_found_end {visited'} (h : captureNextAux σ nfa wf startIdx bit.maxIdx visited [⟨σ.empty, ⟨nfa.start, wf.start_lt⟩, bit, rfl⟩] = (.none, visited')) (h' : ¬bit.hasNext) :
-  captureNext.go σ nfa wf startIdx bit visited = (.none, visited') := by
+theorem captureNext.go_not_found_end {visited'} (h : captureNextAux σ nfa wf startIdx maxIdx visited [⟨σ.empty, ⟨nfa.start, wf.start_lt⟩, bit⟩] = (.none, visited')) (h' : ¬bit.hasNext) :
+  captureNext.go σ nfa wf startIdx maxIdx bit visited = (.none, visited') := by
   unfold captureNext.go
   split <;> simp_all
 
@@ -376,7 +376,7 @@ section
 variable {σ nfa wf it}
 
 theorem captureNext_le (le : it.pos ≤ it.toString.endPos) :
-  captureNext σ nfa wf it = (captureNext.go σ nfa wf it.pos.byteIdx ⟨it, Nat.le_refl _, le⟩ (BitMatrix.zero _ _)).1 := by
+  captureNext σ nfa wf it = (captureNext.go σ nfa wf it.pos.byteIdx it.toString.endPos.byteIdx ⟨it, Nat.le_refl _, le, rfl⟩ (BitMatrix.zero _ _)).1 := by
   simp [captureNext, le]
 
 theorem captureNext_not_le (h : ¬it.pos ≤ it.toString.endPos) :
